chore: pre wip

src/Init/Data/BitVec/Basic.lean
@@ -924,91 +924,44 @@ def extractAndExtendPopulateAux (start : Nat) (x : BitVec w) (acc : List (BitVec
 /-- Given a list of `BitVec w`, we recursively construct the parallel prefix sum for each couple of elements in the initial input. -/
 -- def addVecAux (usedNodes validNodes: Nat) (oldParSum : List (BitVec w)) (newParSum : List (BitVec w)) (heven : usedNodes %2 = 0) (hle : usedNodes ≤ validNodes + 1) (hw : validNodes ≤ w) (hw' : 1 < validNodes) (hlen : oldParSum.length = validNodes) (hlen' : newParSum.length = usedNodes/2) : ListWithLen w ((validNodes + 1)/2) :=
 def addVecAux (usedNodes validNodes: Nat) (oldParSum : List (BitVec w)) (newParSum : List (BitVec w))
-      (heven : usedNodes % 2 = 0) (hin : 1 < inputNodes) (hval : validNodes ≤ inputNodes)
-      (hlen : oldParSum.length = inputNodes)
-      (hlen' : newParSum.length = inputNodes) : List (BitVec w)
--- (hacc :
---   (∀ i (hi : i < newParSum.length) (hl : newParSum.length = usedNodes/2),
---         if hc : i*2 + 1 < oldParSum.length then
---           newParSum.get ⟨i, by simp [hl]; omega⟩ = oldParSum.get ⟨i*2, by omega⟩ + oldParSum.get ⟨i*2 + 1, by omega⟩
---         else
---           newParSum.get ⟨i, by simp [hl]; omega⟩ = oldParSum.get ⟨i*2, by omega⟩)) :
---   {l : List (BitVec w) // (l.length = (validNodes + 1)/2) ∧
---        (∀ i (hi : i < l.length) (hl : l.length = (validNodes + 1)/2),
---         if hc : i*2 + 1 < oldParSum.length then
---           l.get ⟨i, by simp [hl]; omega⟩ = oldParSum.get ⟨i*2, by omega⟩ + oldParSum.get ⟨i*2 + 1, by omega⟩
---         else
---           l.get ⟨i, by simp [hl]; omega⟩ = oldParSum.get ⟨i*2, by omega⟩)
---         }
-  :=
-  match h : validNodes - usedNodes with
-  | 0 => newParSum
-  | n + 1 =>
-      if h : usedNodes + 1 < validNodes then
-        let add := oldParSum.get ⟨usedNodes, by omega⟩ + oldParSum.get ⟨usedNodes + 1, by omega⟩
-        let newVec := newParSum.set ((usedNodes + 1)/2) add
-        -- have : newVec.length = newParSum.length + 1 := by
-        --   have := List.length_concat (as := newParSum) (a := add)
-        --   simp only [List.concat_eq_append, List.length_append, List.length_cons, List.length_nil,
-        --     Nat.zero_add, newVec]
-        addVecAux (usedNodes + 2) validNodes oldParSum newVec (by omega) hin hval hlen (by simp [newVec]; omega)
-            -- (by
-            --   intros i hi hl
-            --   by_cases hlast : i = newVec.length - 1
-            --   · simp [newVec, hlast]
-            --     simp [add]
-            --     split
-            --     · case _ hl' => congr <;> omega
-            --     · case _ hl' => congr <;> omega
-            --   · simp [newVec]
-            --     have := List.getElem_append_left (as := newParSum) (bs := [add]) (i := i) (h := by omega) (h' := by simp; omega)
-            --     rw [this]
-            --     specialize hacc i (by omega) (by omega)
-            --     exact hacc
-            --     )
-      else
-        let add := oldParSum.get ⟨usedNodes, by omega⟩
-        let newVec := newParSum.set ((usedNodes + 1)/2) add
-        addVecAux (usedNodes + 2) validNodes oldParSum newVec (by omega) hin hval hlen (by simp [newVec]; omega)
-          -- (by
-          --   intros i hi hl
-          --   by_cases hlast : i = newVec.length - 1
-          --   · simp [newVec, hlast]
-          --     split
-          --     · case _ hl' => congr <;> omega
-          --     · case _ hl' => congr <;> omega
-          --   · simp [newVec]
-          --     have := List.getElem_append_left (as := newParSum) (bs := [oldParSum[usedNodes]]) (i := i) (h := by omega) (h' := by simp; omega)
-          --     rw [this]
-          --     specialize hacc i (by omega) (by omega)
-          --     exact hacc
-          --   )
-        -- addVecAux (usedNodes + 2) validNodes oldParSum newVec (by omega) (by omega) hw hw' hlen (by omega) (by sorry)
+      (heven : usedNodes % 2 = 0) (hin : 1 < w) (hval : validNodes ≤ w)
+      (hlen : oldParSum.length = w)
+      (hlen' : newParSum.length = w) : {l : List (BitVec w) // l.length = w} :=
+  if h1 : usedNodes < validNodes then
+      if h2 : usedNodes + 1 < validNodes then
+              let add := oldParSum.get ⟨usedNodes, by omega⟩ + oldParSum.get ⟨usedNodes + 1, by omega⟩
+              let newVec := newParSum.set ((usedNodes + 1)/2) add
+              addVecAux (usedNodes + 2) validNodes oldParSum newVec (by omega) hin hval hlen (by simp [newVec]; omega)
+            else
+              let add := oldParSum.get ⟨usedNodes, by omega⟩
+              let newVec := newParSum.set ((usedNodes + 1)/2) add
+              addVecAux (usedNodes + 2) validNodes oldParSum newVec (by omega) hin hval hlen (by simp [newVec]; omega)
+        else
+   ⟨newParSum, by omega⟩
 termination_by (validNodes - usedNodes)
 
 /-- Tail-recursive definition of parrallel sum prefix. At each iteration, we construct a new vector containing the results of summing each couple of elements in the initial vector. -/
 def parPrefixSum
-      (w validNodes inputNodes : Nat) (extBits : List (BitVec w))
-      (hin : 1 < inputNodes) (hval : validNodes ≤ inputNodes)
-      (hlen' : extBits.length = inputNodes) : BitVec w :=
+      (w validNodes : Nat) (extBits : List (BitVec w))
+      (hin : 1 < w) (hval : validNodes ≤ w)
+      (hlen : extBits.length = w) : BitVec w :=
   match h : validNodes - 1 with
   | 0 => extBits.get ⟨0, by omega⟩
   | n' + 1 =>
-    let res := addVecAux 0 validNodes extBits extBits (by omega) (by sorry) (by sorry) (by sorry)
-    -- parPrefixSum w (validNodes := (validNodes + 1)/2)
-    sorry
+    let res := addVecAux 0 validNodes extBits extBits (by omega) hin hval hlen hlen
+    parPrefixSum w (validNodes := (validNodes + 1)/2) res.val hin (by omega) (by omega)
 
-/-- We express `popCount` as the result of parallel prefix sum. -/
-def popCountParSum {x : BitVec w} : BitVec w :=
-  if hw : w = 0 then 0
-  else
-    if hw' : w = 1 then x
-    else
-      let extBits := extractAndExtendPopulateAux 0 x [] (by simp) (by simp) (by simp)
-      have ⟨hlen, hproof⟩ := extBits.property
+-- /-- We express `popCount` as the result of parallel prefix sum. -/
+-- def popCountParSum {x : BitVec w} : BitVec w :=
+--   if hw : w = 0 then 0
+--   else
+--     if hw' : w = 1 then x
+--     else
+--       let extBits := extractAndExtendPopulateAux 0 x [] (by simp) (by simp) (by simp)
+--       have ⟨hlen, hproof⟩ := extBits.property
 
-      sorry
-      -- parPrefixSum (w := w) (validNodes := w) (extBits := extBits.val) (by sorry) (by omega)
+--       sorry
+--       -- parPrefixSum (w := w) (validNodes := w) (extBits := extBits.val) (by sorry) (by omega)
 
 /-- Tail-recursive definition of popcount.
  The bitwidth of `x` explictly boundspop the number of recursions, thus bounding the depth of the circuit as well
@@ -1022,7 +975,7 @@ termination_by (w - n)
 /-- Count the number of bits with value one in a bitvec -/
 def popCount {w : Nat} (x : BitVec w) : BitVec w := popCountAuxRec x 0 0
 
-theorem correctness (x r n : BitVec w) :
-  x.popCount =
+-- theorem correctness (x r n : BitVec w) :
+--   x.popCount =
 
 end BitVec
